# Nabla算法的运算

$$
\nabla(f+g)=\nabla f+\nabla g
$$

$$
\nabla \cdot(\boldsymbol{A}+\boldsymbol{B})=(\boldsymbol{\nabla} \cdot \boldsymbol{A})+(\boldsymbol{\nabla} \cdot \boldsymbol{B}) 
$$

$$
\nabla \times(\boldsymbol{A}+\boldsymbol{B})=(\boldsymbol{\nabla} \times \boldsymbol{A})+(\boldsymbol{\nabla} \times \boldsymbol{B})
$$

$$
\nabla(f g)=f \nabla g+g \nabla f
$$

$$
\nabla(\boldsymbol{A} \cdot \boldsymbol{B})=\boldsymbol{A} \times(\boldsymbol{\nabla} \times \boldsymbol{B})+\boldsymbol{B} \times(\boldsymbol{\nabla} \times \boldsymbol{A})+(\boldsymbol{A} \cdot \boldsymbol{\nabla}) \boldsymbol{B}+(\boldsymbol{B} \cdot \boldsymbol{\nabla}) \boldsymbol{A}
$$

$$
\nabla \cdot(f \boldsymbol{A})=f(\boldsymbol{\nabla} \cdot \boldsymbol{A})+\boldsymbol{A} \cdot(\boldsymbol{\nabla} f)
$$

$$
\nabla \cdot(\boldsymbol{A} \times \boldsymbol{B})=\boldsymbol{B} \cdot(\boldsymbol{\nabla} \times \boldsymbol{A})-\boldsymbol{A} \cdot(\boldsymbol{\nabla} \times \boldsymbol{B})
$$

$$
\nabla \times(f \boldsymbol{A})=f(\nabla \times \boldsymbol{A})-\boldsymbol{A} \times(\nabla f)
$$

$$
\nabla \times(A \times B)=(B \cdot \nabla) A-(A \cdot \nabla) B+A(\nabla \cdot B)-B(\nabla \cdot A)
$$

$$
\nabla \times(\nabla T)=0
$$

$$
\nabla \cdot(\nabla \times v)=0
$$

$$
\nabla \times(\nabla \times v)=\nabla(\nabla \cdot v)-\nabla^{2} v
$$